begin dfa->reg exp

Lerchner/DFA_to_RegExp.thy
@@ -4,26 +4,146 @@ imports
 "$AFP/Regular-Sets/Regular_Exp"   
 begin
 
+
+(** See proof of theorem 3.4 in **)
+(**https://www-2.dc.uba.ar/staff/becher/Hopcroft-Motwani-Ullman-2001.pdf**)
+
 locale dfa =
   fixes n :: nat
   and sigma :: "'a list"
   and nxt :: "nat \<Rightarrow> 'a \<Rightarrow> nat"
-  (* initial state is 0 *)
+  (* initial state is 1 *)
   and Fin :: "nat set"
+  assumes all_states_greater_than_0: "(\<forall>s . s \<in> Fin \<longrightarrow> s > 0) \<and> (\<forall>i a . nxt i a  > 0)"
 begin
-  
-  fun nxts :: "'a list \<Rightarrow> nat \<Rightarrow> nat" where
+
+fun nxts :: "'a list \<Rightarrow> nat \<Rightarrow> nat" where
   "nxts [] q = q" |
   "nxts (a#w) q = nxts w (nxt q a)"
   
-  definition accepted :: "'a list \<Rightarrow> bool" where
-  "accepted w = (nxts w 0 \<in> Fin)"
+definition accepted :: "'a list \<Rightarrow> bool" where
+  "accepted w = (nxts w 1 \<in> Fin)"
   
 (* Your work goes here: *)
 
-definition rexp_of :: "'a rexp" where "rexp_of = undefined"
+type_synonym 'b path = "nat * ('b list) * nat"
+
+definition path_valid :: "'a path \<Rightarrow> bool" where
+  "path_valid p \<longleftrightarrow> (let (i,w,j) = p in  (nxts w i = j))"
+
+fun states_visited :: "'a path \<Rightarrow> nat list" where
+  "states_visited (i, [], j) = []" | 
+  "states_visited (i, a#w, j) = 
+     (let next = nxt i a in 
+      if next = j then [] 
+      else next # states_visited (next, w, j))"
+
+lemma states_visited_gt_0: "x \<in> set (states_visited (i,w,j)) \<Longrightarrow> x >0 "
+  apply(induction w arbitrary:i)
+  apply(auto)
+  by (smt (verit, ccfv_threshold) all_states_greater_than_0 length_pos_if_in_set less_numeral_extra(3) list.size(3) set_ConsD)
+
+lemma states_visited_valid:
+  assumes "path_valid (i,w,j)"
+  shows " (\<exists>xs ys. nxts xs i = k \<and> xs @ ys = w \<and> xs \<noteq> [] \<and> ys \<noteq> []) \<longleftrightarrow> k \<in> set (states_visited (i,w,j)) "
+  sorry
+
+definition path_restricted :: " 'a path \<Rightarrow> nat \<Rightarrow> bool" where
+  "path_restricted p k \<longleftrightarrow> (path_valid p \<and> (\<forall>s. s \<in> set (states_visited p) \<longrightarrow> s \<le> k))"
+
+
+
+
+fun path_goes_through_node :: "'a path \<Rightarrow> nat \<Rightarrow> bool" where
+  "path_goes_through_node p k = (k \<in> set (states_visited p))"
+
+ 
+fun rexp_goes_through_node :: "'a rexp \<Rightarrow> nat \<Rightarrow> bool" where
+  "rexp_goes_through_node rexp k = (\<exists>w \<in> lang rexp. path_goes_through_node (1, w, nxts w 1) k) "
+
+
+ (** todo  missing case y**)
+lemma split_path_at_node:"p = (i, w, j) \<Longrightarrow> path_valid p \<Longrightarrow>  path_goes_through_node p k \<Longrightarrow> \<exists> x y z . (x @ y @ z = w \<and>
+                                                                        \<not> path_goes_through_node (i, x, k) k \<and>
+                                                                        \<not> path_goes_through_node (k, u, j) k)"
+  sorry
+
+
+definition arcs_rexp :: "nat \<Rightarrow> nat \<Rightarrow> 'a rexp" where
+  "arcs_rexp i j =  List.foldr Plus 
+                  (List.map Atom [ a \<leftarrow> sigma. nxt i a = j]) 
+              Zero"
+
+lemma lang_foldr:"lang (List.foldr Plus xs Zero) = \<Union>{lang x | x. x \<in> set xs} "
+proof(induction xs)
+  case Nil
+  then show ?case by simp
+next
+  case (Cons a xs)
+
+ have "\<Union> {lang x |x. x \<in> set (a # xs)} = \<Union> {lang x |x. x \<in> (set xs \<union>  {a})} "
+   by auto
+  also have "... = \<Union> {lang x |x. x \<in> (set xs )} \<union> lang a"
+    by blast
+  then show ?case
+    by (simp add: local.Cons sup_commute) 
+qed
+
+
+lemma arcs_lang:"[a] \<in> lang (arcs_rexp i j) \<longleftrightarrow>  nxt i a = j "
+  unfolding arcs_rexp_def
+  sorry
+
+(** todo start at -1?**)
+fun R:: "nat \<Rightarrow> nat \<Rightarrow> nat \<Rightarrow> 'a rexp " where
+  "R i j 0 = (if i \<noteq> j then arcs_rexp i j else Plus Zero (arcs_rexp i j))" |
+  "R i j (Suc k) = (let R' = R i j k in
+                           if \<not>rexp_goes_through_node R' k then 
+                              R'
+                           else
+                              let u = R    i    (Suc k) k in
+                              let v = R (Suc k) (Suc k) k in
+                              let w = R (Suc k)    j    k in
+                              Plus  R' (Times u (Times (Star v) w)))"
+
+
+
+
+
+
+lemma " path_restricted (i, w, j) k \<Longrightarrow> w \<in> lang (R i j k)"
+proof(induction k arbitrary: i j)
+  case 0
+
+  then  show ?case 
+
+  proof(cases "i=j")
+    case True
+    then show ?thesis 
+      unfolding path_restricted_def path_valid_def 
+      apply(auto)
+      sorry
+  next
+    case False
+    then show ?thesis sorry
+  qed
+next
+  case (Suc k)
+  then show ?case sorry
+qed
+
+
+  
+definition rexp_of :: "'a rexp" where
+"rexp_of = List.foldr Plus 
+             [ R 0 j n . j \<leftarrow> sorted_list_of_set Fin]
+           Zero"
 
 theorem "w \<in> lang (rexp_of) \<longleftrightarrow> accepted w"
   sorry
+
+end
+
+
 
 end
