Lerchner/DFA_Locale_simple.thy
@@ -1,0 +1,123 @@
+theory DFA_Locale_simple
+imports
+  "$AFP/Regular-Sets/Regular_Exp"
+begin
+
+(* 
+  This theory file defines the basic DFA (Deterministic Finite Automaton) structure
+  using Isabelle's locale mechanism. The DFA is represented with:
+  - n: total number of states
+  - S: set of states (numbered 1 to n)
+  - sigma: alphabet as a list of symbols
+  - nxt: transition function
+  - Fin: set of accepting states
+*)
+locale dfa =
+  fixes 
+    n :: nat           (* Number of states *)
+    and S :: "nat set" (* Set of states *)
+    and sigma :: "'a list"  (* Alphabet *)
+    and nxt :: "nat \<Rightarrow> 'a \<Rightarrow> nat"  (* Transition function *)
+    and Fin :: "nat set"    (* Set of accepting states *)
+
+  assumes 
+    "n > 0"  (* At least one state *)
+    and state_set_def: "S = {1..n}"  (* States are numbered 1 to n *)
+    and states_subset: "Fin \<subseteq> S"     (* All accepting states are valid states *)
+    and transitions_in_S: "\<And>i a. i \<in> S \<longrightarrow> nxt i a \<in> S"  (* Transitions stay within valid states *)
+    and transitions_valid: "nxt i a = j \<Longrightarrow> a \<in> set sigma"  (* Transitions use valid symbols *)
+begin
+
+(* Basic lemma showing that starting state exists in S *)
+lemma start_exist: "1 \<in> S"
+  by (metis atLeastAtMost_iff dfa_axioms dfa_def leI less_one not_gr_zero)
+
+(* Extended transition function for words *)
+fun nxts :: "'a list \<Rightarrow> nat \<Rightarrow> nat" where
+  "nxts [] q = q" |
+  "nxts (a#w) q = nxts w (nxt q a)"
+  
+(* Word acceptance predicate *)
+definition accepted :: "'a list \<Rightarrow> bool" where
+  "accepted w = (nxts w 1 \<in> Fin)"
+
+(* Predicate for paths between states *)
+definition word_run_from_i_j :: "'a list \<Rightarrow> nat \<Rightarrow> nat \<Rightarrow> bool" where
+  "word_run_from_i_j w i j = (nxts w i = j)"
+
+
+
+
+
+
+(* 
+  Path-related operations and lemmas including:
+  - path_of_word: Computes the sequence of states visited by a word
+  - intermediate_path: Gets internal states of a path
+  - paths_between: Set of all paths between two states
+*)
+
+(* Compute sequence of states visited by a word *)
+fun path_of_word :: "'a list \<Rightarrow> nat \<Rightarrow> nat list" where
+  "path_of_word [] i = [i]" |
+  "path_of_word (a#w) i = i # path_of_word w (nxt i a)"
+
+lemma length_of_path:"length (path_of_word w i) = length w + 1"
+  apply(induction w arbitrary:i)
+  apply(auto)
+  done
+
+(* All states in a path must be valid states *)
+lemma path_in_S: "i \<in> S \<Longrightarrow> set (path_of_word w i) \<subseteq> S"
+  apply(induction w arbitrary: i)
+  apply(auto)
+  by (meson in_mono transitions_in_S)
+
+(* Get internal states of a path (excluding start and end) *)
+fun intermediate_path :: "nat list \<Rightarrow> nat list" where
+  "intermediate_path p = butlast (tl p)"
+
+(* Simple lemma about intermediate path computation *)
+lemma intermediate_effect: "intermediate_path (a # is @ [e]) = is"
+  by simp
+
+(* Set of all paths between two states *)
+definition paths_between :: "nat \<Rightarrow> nat \<Rightarrow> (nat list) set" where
+  "paths_between i j = {path_of_word w i | w. word_run_from_i_j w i j}"
+
+
+(*
+  Operations and lemmas for paths with restrictions on intermediate states:
+  - intermediate_path_restricted: Predicate for paths with bounded intermediate states
+  - restricetd_paths_between: Set of paths with bounded intermediate states
+*)
+
+(* Predicate for paths where intermediate nodes are bounded *)
+definition intermediate_path_restricted :: "nat list \<Rightarrow> nat \<Rightarrow> bool" where
+  "intermediate_path_restricted p k = (\<forall>s. s \<in> set (intermediate_path p) \<longrightarrow> s \<le> k)"
+
+(* Set of paths between states with bounded intermediate nodes *)
+definition restricetd_paths_between :: "nat \<Rightarrow> nat \<Rightarrow> nat \<Rightarrow> (nat list) set" where
+  "restricetd_paths_between i j k = {p. p \<in> paths_between i j \<and> intermediate_path_restricted p k}"
+
+(* All paths are automatically restricted by n *)
+corollary path_word_restricted_n: 
+  "i \<in> S \<Longrightarrow> j \<in> S \<Longrightarrow> paths_between i j = restricetd_paths_between i j n"
+  unfolding restricetd_paths_between_def paths_between_def intermediate_path_restricted_def
+  apply(auto)
+  by (metis atLeastAtMost_iff in_mono in_set_butlastD list.sel(2) list.set_sel(2) 
+        path_in_S state_set_def)
+
+(* Intermediate states are subset of all states in path *)
+lemma intermediate_smaller: "set (intermediate_path p) \<subseteq> set p"
+  apply(auto)
+  by (metis in_set_butlastD list.sel(2) list.set_sel(2))
+
+(* All paths starting from valid states are restricted by n *)
+corollary restricted_n: "i\<in> S \<Longrightarrow> intermediate_path_restricted (path_of_word w i) n"
+  unfolding intermediate_path_restricted_def
+  by (metis atLeastAtMost_iff in_mono intermediate_smaller path_in_S state_set_def)
+
+
+end
+end
