Lerchner/DFA_to_RegExp2.thy
@@ -1,0 +1,173 @@
+theory DFA_to_RegExp2
+
+imports "DFA_Locale_simple"
+begin
+
+
+(** See proof of theorem 3.4 in **)
+(**https://www-2.dc.uba.ar/staff/becher/Hopcroft-Motwani-Ullman-2001.pdf**)
+
+context dfa begin
+
+
+lemma lang_combine_plus:"lang (List.foldr Plus xs Zero) = \<Union>{lang x | x. x \<in> set xs}"
+  apply(induction xs)
+  apply(auto)
+  done
+
+
+definition arcs_rexp :: "nat \<Rightarrow> nat \<Rightarrow> 'a rexp" where
+   "arcs_rexp i j = foldr Plus [Atom a . a \<leftarrow> sigma, nxt i a = j] Zero"
+
+definition rexp_goes_through_node :: "'a rexp \<Rightarrow> nat  \<Rightarrow> nat \<Rightarrow> bool" where
+  "rexp_goes_through_node r i k = (\<exists>w \<in> lang r.  k \<in> set (path_of_word w i))"
+
+
+(** todo start at -1?**)
+fun R:: "nat \<Rightarrow> nat \<Rightarrow> nat \<Rightarrow> 'a rexp " where
+  "R i j 0 = (if i \<noteq> j then arcs_rexp i j else Plus One (arcs_rexp i j))" |
+  "R i j (Suc k) = (let R' = R i j k in
+                           if \<not>rexp_goes_through_node R' k i then 
+                              R'
+                           else
+                              let u = R    i    (Suc k) k in
+                              let v = R (Suc k) (Suc k) k in
+                              let w = R (Suc k)    j    k in
+                              Plus  R' (Times u (Times (Star v) w)))"
+
+
+
+
+lemma lang_arcs_rexp:" lang (arcs_rexp i j) = { [a] | a.  nxt i a = j}"
+proof -
+    have " lang (arcs_rexp i j) = lang (foldr Plus [Atom a . a \<leftarrow> sigma, nxt i a = j] Zero)"
+      by (simp add: arcs_rexp_def)
+    also have "... = \<Union>{lang x | x. x \<in> set [Atom a . a \<leftarrow> sigma, nxt i a = j]}"
+      using lang_combine_plus by blast
+    also have "... = \<Union>{lang x | x. x \<in> {Atom a | a. a \<in> set sigma \<and> nxt i a = j}}"
+      by auto
+    also have "... = \<Union>{ lang (Atom a) | a. a \<in> set sigma \<and> nxt i a = j}"
+      by blast
+    also have "... =  { [a] | a. a \<in> set sigma \<and> nxt i a = j}"
+      by(auto)
+    also have "... =  { [a] | a.  nxt i a = j}"
+      by (simp add: transitions_valid)
+    finally show ?thesis 
+      by auto
+  qed
+
+lemma Rmono: "lang (R i j k) \<subseteq> lang (R i j (k + 1))"
+  apply(cases "rexp_goes_through_node ( R i j k) k i")
+  by(auto)
+
+lemma lang_Rij0:" lang (R i j 0) = { [a] | a.  nxt i a = j}  \<union> (if i = j then {[]} else {})"
+   by (simp add: lang_arcs_rexp)
+
+
+lemma path_Rij0:" w\<in> lang (R i j 0) \<Longrightarrow> path_of_word w i = (if w=[] then [i] else [i,j])"
+proof -
+  assume "w\<in> lang (R i j 0)"
+  then have "w \<in> { [a] | a.  nxt i a = j}  \<union> (if i = j then {[]} else {})"
+    using lang_Rij0 by fastforce
+  then show "path_of_word w i = (if w=[] then [i] else [i,j])"
+    apply(cases "i=j")
+    by(auto)
+qed
+
+
+lemma no_intermediate_path_k0:"i \<in> S\<Longrightarrow> p = (path_of_word w i) \<Longrightarrow>  intermediate_path_restricted p 0 \<Longrightarrow> intermediate_path p = [] "
+  unfolding  intermediate_path_restricted_def
+  by (metis atLeastAtMost_iff dual_order.trans intermediate_smaller list.exhaust list.set_intros(1) not_one_le_zero path_in_S state_set_def subset_iff)
+
+lemma path_shape_no_intermediate:"i \<in> S \<Longrightarrow> intermediate_path (path_of_word w i) = [] \<Longrightarrow> path_of_word w i = (if w=[] then [i] else [i,nxt i (hd w)])"
+  unfolding word_run_from_i_j_def
+  apply(induction w arbitrary:i)
+  apply(auto)
+  by (metis butlast.simps(2) butlast_tl list.discI list.sel(2) transitions_in_S)
+
+lemma langR1j0_1:
+  assumes "w \<in> lang (R i j 0)"
+  shows "(word_run_from_i_j w i j \<and>  intermediate_path_restricted (path_of_word w i) 0)"
+  using assms unfolding word_run_from_i_j_def intermediate_path_restricted_def 
+  apply(cases "i=j")
+  by(auto simp add:lang_arcs_rexp)
+
+lemma langR1j0_2:
+  assumes "i \<in> S"
+  and "word_run_from_i_j w i j" and "intermediate_path_restricted (path_of_word w i) 0"
+  shows "w \<in> lang (R i j 0)"
+using assms proof -
+   have "intermediate_path (path_of_word w i) = []"
+    using assms no_intermediate_path_k0 by auto
+
+  then have "path_of_word w i  =(if w=[] then [i] else [i,nxt i (hd w)])"
+    using assms path_shape_no_intermediate by auto
+
+  then have "w = (if w=[] then [] else [hd w])"
+    by (metis list.distinct(1) list.inject list.sel(1) path_of_word.elims)
+
+  then consider "w=[]" | "w=[hd w]"
+    by meson
+  then show "w \<in> lang (R i j 0)"
+    apply(cases)
+    apply(auto simp add:lang_Rij0 lang_arcs_rexp)
+    using assms word_run_from_i_j_def apply auto
+    by (metis nxts.simps(1) nxts.simps(2) ) +
+qed
+
+
+
+
+lemma langRijk: 
+  assumes "i \<in> S  \<and> j \<in> S "
+  shows"  w \<in> lang (R i j k) =  (word_run_from_i_j w i j \<and>  intermediate_path_restricted (path_of_word w i) k)"
+using assms proof(induction k arbitrary: i)
+  case 0
+  then show ?case
+    using langR1j0_1 langR1j0_2 by blast
+
+next
+  case (Suc k)
+
+  show ?case 
+    sorry
+
+qed
+ 
+
+
+
+
+corollary langRn: "i \<in> S \<Longrightarrow> j \<in> S \<Longrightarrow> w \<in> lang (R i j n) \<longleftrightarrow>   word_run_from_i_j w i j"
+  using langRijk restricted_n by auto
+
+
+definition rexp_of :: "'a rexp" where
+"rexp_of = List.foldr Plus 
+             [ R 1 j n . j \<leftarrow> sorted_list_of_set Fin]
+           Zero"
+
+theorem "w \<in> lang (rexp_of) \<longleftrightarrow> accepted w"
+proof -
+  have f:"finite S"
+    by (simp add: state_set_def)
+
+  have "lang (rexp_of) = \<Union>{lang x | x. x \<in> set [ R 1 j n . j \<leftarrow> sorted_list_of_set Fin]}"
+    by (simp add: lang_combine_plus rexp_of_def)
+  also have "... = \<Union>{lang (R 1 j n) | j. j \<in> Fin} "
+    using f finite_subset states_subset by fastforce
+  also have "... = {w.  (\<exists>j \<in> Fin. w \<in> lang (R 1 j n))  }"
+    by blast
+   also have "... = {w.  (\<exists>j \<in> Fin. word_run_from_i_j w 1 j)  }"
+     by (metis in_mono start_exist states_subset langRn)
+  also have "...= {w. accepted w }"
+    using accepted_def word_run_from_i_j_def by auto
+  ultimately show ?thesis
+    by simp
+qed
+
+end
+
+
+
+end
