Lerchner/test.thy
@@ -1,0 +1,151 @@
+theory test
+  imports Main HOL.List DFA_to_RegExp
+begin
+
+locale dfa =
+  fixes n :: nat
+  and sigma :: "'a list"
+  and nxt :: "nat \<Rightarrow> 'a \<Rightarrow> nat"
+  and Fin :: "nat set"
+begin
+  
+fun nxts :: "'a list \<Rightarrow> nat \<Rightarrow> nat" where
+  "nxts [] q = q" |
+  "nxts (a#w) q = nxts w (nxt q a)"
+  
+definition accepted :: "'a list \<Rightarrow> bool" where
+  "accepted w = (nxts w 0 \<in> Fin)"
+
+fun list_to_rexp :: "'a list \<Rightarrow> 'a rexp" where
+  "list_to_rexp [] = Zero" |
+  "list_to_rexp [x] = Atom x" |
+  "list_to_rexp (x#xs) = Plus (Atom x) (list_to_rexp xs)"
+
+definition arc :: "nat \<Rightarrow> nat \<Rightarrow> 'a rexp" where
+  "arc i j = list_to_rexp [a \<leftarrow> sigma. nxt i a = j]"
+
+(* Test instance *)
+definition test_sigma :: "string list"
+where "test_sigma = [''a'', ''b'']"
+
+fun test_nxt :: "nat \<Rightarrow> string \<Rightarrow> nat" where
+  "test_nxt 0 ''a'' = 1" |
+  "test_nxt 0 ''b'' = 0" |
+  "test_nxt (Suc 0) ''a'' = 1" |
+  "test_nxt (Suc 0) ''b'' = 0"
+
+definition test_Fin :: "nat set"
+where "test_Fin = {1}"
+
+(* Test cases *)
+lemma "arc 0 1 = list_to_rexp [''a'']"
+  by (simp add: arc_def test_sigma_def)
+
+lemma "arc 0 0 = list_to_rexp [''b'']"
+  by (simp add: arc_def test_sigma_def)
+
+lemma "arc 1 1 = list_to_rexp [''a'']"
+  by (simp add: arc_def test_sigma_def)
+
+end
+
+end
+
+
+lemma start_exist: "1 \<in> S"
+   by (metis atLeastAtMost_iff dfa_axioms dfa_def leI less_one not_gr_zero)
+
+
+fun nxts :: "'a list \<Rightarrow> nat \<Rightarrow> nat" where
+  "nxts [] q = q" |
+  "nxts (a#w) q = nxts w (nxt q a)"
+  
+definition accepted :: "'a list \<Rightarrow> bool" where
+  "accepted w = (nxts w 1 \<in> Fin)"
+
+definition word_run_from_i_j :: "'a list \<Rightarrow> nat \<Rightarrow> nat \<Rightarrow> bool" where
+  "word_run_from_i_j w i j =  (nxts w i = j)"
+
+
+corollary accepted_run:"accepted xs = (\<exists>j\<in> Fin. word_run_from_i_j xs 1 j) "
+  by (simp add: accepted_def word_run_from_i_j_def)
+
+(* Your work goes here: *)
+
+
+
+
+(** The traversed states of a word w. **)
+fun path_of_word :: "'a list \<Rightarrow> nat  \<Rightarrow> nat list" where
+  "path_of_word [] i = [i]" |
+  "path_of_word (a#w) i = i # path_of_word w (nxt i a) "
+
+lemma path_in_S:"i \<in> S \<Longrightarrow> set (path_of_word w i) \<subseteq> S"
+  apply(induction w arbitrary: i)
+  apply(auto)
+  by (meson in_mono transitions_in_S)
+
+
+
+fun intermediate_path:: "nat list \<Rightarrow> nat list" where
+  "intermediate_path p = butlast (tl p)"
+
+lemma intermediate_effect:"intermediate_path (a # is @ [e]) = is"
+  by simp
+
+definition paths_between :: "nat \<Rightarrow> nat  \<Rightarrow> (nat list) set" where
+  "paths_between i j = {path_of_word w i | w . word_run_from_i_j w i j}"
+
+(** The intermediate path consists of all nodes except the first and last nodes. **)
+definition intermediate_path_restricted :: "nat list \<Rightarrow> nat  \<Rightarrow> bool" where
+  "intermediate_path_restricted p k = (\<forall>s. s \<in> set (intermediate_path p) \<longrightarrow> s \<le> k)"
+
+
+(** A path is restricted to a node k if no intermediate node in the path is greater than k. **)
+definition restricetd_paths_between :: "nat \<Rightarrow> nat \<Rightarrow> nat \<Rightarrow> (nat list) set" where
+  "restricetd_paths_between i j k = {p. p \<in> paths_between i j \<and> intermediate_path_restricted p k}"
+
+
+corollary path_word_restricted_n:"i \<in> S \<Longrightarrow> j \<in> S  \<Longrightarrow>paths_between i j = restricetd_paths_between i j n"
+  unfolding restricetd_paths_between_def paths_between_def intermediate_path_restricted_def
+  apply(auto)
+  by (metis atLeastAtMost_iff in_mono in_set_butlastD list.sel(2) list.set_sel(2) path_in_S state_set_def)
+
+
+lemma intermediate_smaller: "set (intermediate_path p) \<subseteq> set p"
+  apply(auto)
+  by (metis in_set_butlastD list.sel(2) list.set_sel(2))
+
+corollary restricted_n:"i\<in> S \<Longrightarrow> intermediate_path_restricted (path_of_word w i) n"
+  unfolding intermediate_path_restricted_def
+  by (metis atLeastAtMost_iff in_mono intermediate_smaller path_in_S state_set_def)
+ 
+
+(** somehow this is necessery for automation **)
+lemma x:"\<Union>{lang x | x. x \<in> set (map A xs)} = \<Union>{ lang (A x) | x. x \<in> set (xs)} "
+  by auto
+
+lemma path_restricted_mono:"intermediate_path_restricted xs k \<Longrightarrow> intermediate_path_restricted xs (k+1)"
+  unfolding intermediate_path_restricted_def
+  apply(auto)
+  done
+
+
+  
+ 
+(** Util **)
+
+lemma accepted_path_k:"word_run_from_i_j w k j = (last (path_of_word w k) = j)"
+  apply(induction w k rule: path_of_word.induct)
+  apply(auto simp add:word_run_from_i_j_def)
+  using dfa.path_of_word.elims dfa_axioms apply blast
+  using dfa.path_of_word.elims dfa_axioms by blast
+
+corollary accepted_path:"accepted w  = (\<exists>j \<in> Fin. word_run_from_i_j w 1 j)"
+  unfolding accepted_def word_run_from_i_j_def
+  by(auto)
+
+
+
+
+end
